NuBasicAbstractors.thy
@@ -5,14 +5,14 @@ begin
 text \<open>Basic \<nu>-abstractors\<close>
 
 text \<open>Examples for automatic property inference\<close>
-schematic_goal [simplified]: "Nu_Share (\<bool> \<nuFusion> \<nat>['b :: len] \<nuFusion> \<bool>) ?set ?sh" by (rule \<nu>share)+
-schematic_goal [simplified]: "Nu_Share N s f \<Longrightarrow> Nu_Share (N \<nuFusion> N \<nuFusion> N) ?set ?sh" for N :: "('a::sharable_lrep, 'b) nu"
-  including show_more1 by (blast intro: \<nu>share)
-schematic_goal [simplified]: "\<nu>Equalable (\<bool> \<nuFusion> \<nat>['b :: len] \<nuFusion> \<nat>['a :: len]) ?ceq" by (rule \<nu>equable)+
-schematic_goal [simplified]: "\<nu>Disposable ((b,x,y) \<tycolon> \<bool> \<nuFusion> \<nat>['b :: len] \<nuFusion> \<nat>['a :: len])" by (rule \<nu>disposable)+
+schematic_goal [simplified]: "\<nu>Share (\<bool> \<nuFusion> \<nat>['b :: len] \<nuFusion> \<bool>) ?set ?sh" by (rule \<nu>intro)+
+(* schematic_goal [simplified]: "\<nu>Share N s f \<Longrightarrow> \<nu>Share (N \<nuFusion> N \<nuFusion> N) ?set ?sh" for N :: "('a::sharable_lrep, 'b) nu"
+  including show_more1 by (blast intro: \<nu>intro Premise_I) *)
+schematic_goal [simplified]: "\<nu>Equalable (\<bool> \<nuFusion> \<nat>['b :: len] \<nuFusion> \<nat>['a :: len]) ?ceq" by (rule \<nu>intro)+
+schematic_goal [simplified]: "\<nu>Disposable ((b,x,y) \<tycolon> \<bool> \<nuFusion> \<nat>['b :: len] \<nuFusion> \<nat>['a :: len])" by (rule \<nu>intro)+
 ML_val \<open>
 val tm2 = Syntax.read_prop (Proof_Context.set_mode Proof_Context.mode_schematic @{context})
-    "Nu_Share N s f \<Longrightarrow> Nu_Share (N \<nuFusion> N \<nuFusion> N) ?set ?sh"
+    "\<nu>Share N s f \<Longrightarrow> \<nu>Share (N \<nuFusion> N \<nuFusion> N) ?set ?sh"
   |> Thm.cterm_of @{context}
 val tm = Thm.cprop_of @{thm th1}
 val th = Goal.init tm2
@@ -27,9 +27,9 @@ definition NuRefine :: " ('a :: lrep, 'b) nu \<Rightarrow> 'b set \<Rightarrow> 
   where "N \<nuRefine> T = Nu (\<lambda>(p,x). x \<in> T \<and>(p \<nuLinkL> N \<nuLinkR> x))"
 lemma [simp]: "p \<nuLinkL> N \<nuRefine> P \<nuLinkR> x \<longleftrightarrow> x \<in> P \<and> (p \<nuLinkL> N \<nuLinkR> x)" unfolding NuRefine_def by auto
 lemma [elim]: "x \<ratio> N \<nuRefine> P \<Longrightarrow> (x \<in> P \<Longrightarrow> x \<ratio> N \<Longrightarrow> C) \<Longrightarrow> C" unfolding Inhabited_def by auto
-lemma [\<nu>cast]: "\<^bold>c\<^bold>a\<^bold>s\<^bold>t x \<tycolon> N \<nuRefine> P \<longmapsto> x \<tycolon> N \<^bold>m\<^bold>e\<^bold>a\<^bold>n\<^bold>w\<^bold>h\<^bold>i\<^bold>l\<^bold>e x \<in> P" unfolding Cast_def by auto
+lemma [\<nu>intro]: "\<^bold>c\<^bold>a\<^bold>s\<^bold>t x \<tycolon> N \<longmapsto> Y \<^bold>m\<^bold>e\<^bold>a\<^bold>n\<^bold>w\<^bold>h\<^bold>i\<^bold>l\<^bold>e Q \<Longrightarrow> \<^bold>c\<^bold>a\<^bold>s\<^bold>t x \<tycolon> N \<nuRefine> P \<longmapsto> Y \<^bold>m\<^bold>e\<^bold>a\<^bold>n\<^bold>w\<^bold>h\<^bold>i\<^bold>l\<^bold>e Q \<and>x \<in> P" unfolding Cast_def by auto
 
-section \<open>Others\<close>
+(* section \<open>Others\<close>
 
 definition stepin :: "( ('a::lrep) \<Rightarrow> ('b::lrep) state) \<Rightarrow> ( ('c::lrep) \<times> 'a \<Rightarrow> ('c \<times> 'b) state)"
   where "stepin f x = (case x of (c,a) \<Rightarrow> bind (f a) (\<lambda>y. StatOn (c,y)))"
@@ -57,9 +57,9 @@ thm \<nu>auto_construct
 
 ML \<open>@{term "29::32"}\<close>
 lemma [simplified]: "(10::3) = (0::3)"  by auto
-  thm term_def
+  thm term_def *)
 
-schematic_goal [simplified]:"\<^bold>c\<^bold>a\<^bold>s\<^bold>t (A\<heavy_comma>B\<heavy_comma>(x \<tycolon> C \<nuRefine> P)\<heavy_comma>D) \<longmapsto> (A\<heavy_comma>B\<heavy_comma>x \<tycolon> C\<heavy_comma>D) \<^bold>m\<^bold>e\<^bold>a\<^bold>n\<^bold>w\<^bold>h\<^bold>i\<^bold>l\<^bold>e ?P" by (rule \<nu>cast)+
-schematic_goal "\<^bold>c\<^bold>a\<^bold>s\<^bold>t (A\<heavy_comma>B) \<longmapsto> (A\<heavy_comma>B) \<^bold>m\<^bold>e\<^bold>a\<^bold>n\<^bold>w\<^bold>h\<^bold>i\<^bold>l\<^bold>e ?P" by (rule \<nu>cast)
+schematic_goal [simplified]:"\<^bold>c\<^bold>a\<^bold>s\<^bold>t (A\<heavy_comma>B\<heavy_comma>(x \<tycolon> C \<nuRefine> P)\<heavy_comma>D) \<longmapsto> (A\<heavy_comma>B\<heavy_comma>x \<tycolon> C\<heavy_comma>D) \<^bold>m\<^bold>e\<^bold>a\<^bold>n\<^bold>w\<^bold>h\<^bold>i\<^bold>l\<^bold>e ?P" by (rule \<nu>intro)+
+schematic_goal "\<^bold>c\<^bold>a\<^bold>s\<^bold>t (A\<heavy_comma>B) \<longmapsto> (A\<heavy_comma>B) \<^bold>m\<^bold>e\<^bold>a\<^bold>n\<^bold>w\<^bold>h\<^bold>i\<^bold>l\<^bold>e ?P" by (rule \<nu>intro)
 
 end
